thys/Common_Rec_Corec/Comodels.thy
@@ -2,21 +2,24 @@ theory Comodels
   imports "Expressions"
 begin(* *)
  
-definition dtorNeC :: "('E' \<Rightarrow> (('a::var,'a,'E','E')G) set + 'a E) \<Rightarrow> bool" where 
-"dtorNeC dtor \<equiv> \<forall>e U. dtor e = Inl U \<longrightarrow> U \<noteq> {}"
+definition dtorNeC :: "('E' \<Rightarrow> bool) \<Rightarrow> ('E' \<Rightarrow> (('a::var,'a,'E','E')G) set + 'a E) \<Rightarrow> bool" where 
+"dtorNeC valid dtor \<equiv> \<forall>e U. valid e \<and> dtor e = Inl U \<longrightarrow> U \<noteq> {}"
 
-definition dtorPermC :: "('E' \<Rightarrow> (('a::var,'a,'E','E')G) set + 'a E) \<Rightarrow> (('a \<Rightarrow> 'a) \<Rightarrow> 'E' \<Rightarrow> 'E') \<Rightarrow> bool" 
-where "dtorPermC dtor perm \<equiv> 
-\<forall>\<sigma> e. small \<sigma> \<and> bij \<sigma> \<longrightarrow> 
+definition dtorPermC :: "('E' \<Rightarrow> bool) \<Rightarrow> 
+('E' \<Rightarrow> (('a::var,'a,'E','E')G) set + 'a E) \<Rightarrow> 
+(('a \<Rightarrow> 'a) \<Rightarrow> 'E' \<Rightarrow> 'E') \<Rightarrow> bool" 
+where "dtorPermC valid dtor perm \<equiv> 
+\<forall>\<sigma> e. valid e \<and> small \<sigma> \<and> bij \<sigma> \<longrightarrow> 
   (\<forall> U. dtor e = Inl U \<longrightarrow> (\<exists>U'. dtor (perm \<sigma> e) = Inl U' \<and> U' \<subseteq> Gren \<sigma> \<sigma> ` (Gmap (perm \<sigma>) (perm \<sigma>) ` U)))
   \<and> 
   (\<forall>e1. dtor e = Inr e1 \<longrightarrow> (\<exists>e1'. dtor (perm \<sigma> e) = Inr e1' \<and> e1' =  Eperm \<sigma> e1))"
 
-definition dtorVrsGrenC :: "('E' \<Rightarrow> (('a::var,'a,'E','E')G) set + 'a E) \<Rightarrow> 
-  (('a \<Rightarrow> 'a) \<Rightarrow> 'E' \<Rightarrow> 'E') \<Rightarrow> ('E' \<Rightarrow> 'a set) \<Rightarrow> bool" 
+definition dtorVrsGrenC :: "('E' \<Rightarrow> bool) \<Rightarrow> 
+('E' \<Rightarrow> (('a::var,'a,'E','E')G) set + 'a E) \<Rightarrow> 
+(('a \<Rightarrow> 'a) \<Rightarrow> 'E' \<Rightarrow> 'E') \<Rightarrow> ('E' \<Rightarrow> 'a set) \<Rightarrow> bool" 
 where
-"dtorVrsGrenC dtor perm Vrs \<equiv> 
- (\<forall>e U u1 u2. dtor e = Inl U \<and> {u1,u2} \<subseteq> U \<longrightarrow> 
+"dtorVrsGrenC valid dtor perm Vrs \<equiv> 
+ (\<forall>e U u1 u2. valid e \<and> dtor e = Inl U \<and> {u1,u2} \<subseteq> U \<longrightarrow> 
    (\<exists>\<sigma>. small \<sigma> \<and> bij \<sigma> \<and> 
         id_on ((\<Union> (Vrs ` GSupp1 u1) - GVrs2 u1)) \<sigma> \<and> 
         Gren id \<sigma> (Gmap (perm \<sigma>) id u1) = u2))"
@@ -28,10 +31,12 @@ Ector_eqA: "\<And>u1 u2. Ector u1 = Ector u2 \<Longrightarrow>
      Gren id \<sigma> (Gmap (Eperm \<sigma>) (Eperm \<sigma>) u1) = u2)"
 *)
 
-definition dtorVrsC :: "('E' \<Rightarrow> (('a::var,'a,'E','E')G) set + 'a E) \<Rightarrow> ('E' \<Rightarrow> 'a set) \<Rightarrow> bool" 
+definition dtorVrsC :: "('E' \<Rightarrow> bool) \<Rightarrow> 
+('E' \<Rightarrow> (('a::var,'a,'E','E')G) set + 'a E) \<Rightarrow> 
+('E' \<Rightarrow> 'a set) \<Rightarrow> bool" 
 where
-"dtorVrsC dtor Vrs \<equiv> 
- (\<forall>e.  
+"dtorVrsC valid dtor Vrs \<equiv> 
+ (\<forall>e. valid e \<longrightarrow>   
   (\<forall>U. dtor e = Inl U \<longrightarrow> 
        (\<forall>u\<in>U. GVrs1 u \<union> 
               (\<Union> {Vrs e - GVrs2 u | e . e \<in> GSupp1 u}) \<union> 
@@ -42,22 +47,39 @@ where
   (\<forall>e1. dtor e = Inr e1 \<longrightarrow> EVrs e1 \<subseteq> Vrs e)
 )"
 
+(* destructor preserves validity *)
+definition presDV :: "('E' \<Rightarrow> bool) \<Rightarrow> 
+  ('E' \<Rightarrow> (('a::var,'a,'E','E')G) set + 'a E) \<Rightarrow> bool" 
+where "presDV valid dtor \<equiv> 
+ \<forall>e. valid e \<longrightarrow>   
+     (\<forall>U u e'. dtor e = Inl U \<and> u \<in> U \<and> e' \<in> GSupp1 u \<union> GSupp2 u \<longrightarrow> valid e')"
+
+(* permutation preserves validity *)
+definition presPV :: "('E' \<Rightarrow> bool) \<Rightarrow> (('a::var \<Rightarrow> 'a) \<Rightarrow> 'E' \<Rightarrow> 'E') \<Rightarrow> bool" 
+where "presPV valid perm \<equiv> 
+\<forall>\<sigma> e. valid e \<and> small \<sigma> \<and> bij \<sigma> \<longrightarrow> valid (perm \<sigma> e)"
+
 (* Full-recursion comodel:   *)
 locale Comodel =
 fixes (* no set V, as we need no Barendregt convention here *)
+Evalid' :: "'E' \<Rightarrow> bool" and 
 Edtor' :: "'E' \<Rightarrow> (('a::var,'a,'E','E')G) set + 'a E" 
 and Eperm' :: "('a::var \<Rightarrow> 'a) \<Rightarrow> 'E' \<Rightarrow> 'E'" 
 and EVrs' :: "'E' \<Rightarrow> 'a::var set" 
 assumes 
-nom: "nom Eperm' EVrs'" 
+presDV_Evalid'_Edtor': "presDV Evalid' Edtor'"
+and 
+presPV_Evalid'_Edtor': "presPV Evalid' Eperm'"
+and
+nom: "nom Evalid' Eperm' EVrs'" 
 and  
-dtorNeC: "dtorNeC Edtor'"
+dtorNeC: "dtorNeC Evalid' Edtor'"
 and 
-dtorPermC: "dtorPermC Edtor' Eperm'"
+dtorPermC: "dtorPermC Evalid' Edtor' Eperm'"
 and 
-dtorVrsGrenC: "dtorVrsGrenC Edtor' Eperm' EVrs'"
+dtorVrsGrenC: "dtorVrsGrenC Evalid' Edtor' Eperm' EVrs'"
 and 
-dtorVrsC: "dtorVrsC Edtor' EVrs'"
+dtorVrsC: "dtorVrsC Evalid' Edtor' EVrs'"
 begin 
 
 
@@ -65,26 +87,27 @@ definition corec :: "'E' \<Rightarrow> 'a E" where
 "corec = undefined"
 
 lemma corec_Edtor_Inl:
-"Edtor' e = Inl U \<Longrightarrow> Gmap corec corec ` U  \<subseteq> Edtor (corec e)"
+"Evalid' e \<Longrightarrow> Edtor' e = Inl U \<Longrightarrow> Gmap corec corec ` U  \<subseteq> Edtor (corec e)"
 sorry
 
 lemma corec_Edtor_Inr:
-"Edtor' e = Inr e1 \<Longrightarrow> corec e = e1"
+"Evalid' e \<Longrightarrow> Edtor' e = Inr e1 \<Longrightarrow> corec e = e1"
 sorry
 
 lemma corec_Eperm:
-"small \<sigma> \<Longrightarrow> bij \<sigma> \<Longrightarrow>   
- corec (Eperm' \<sigma> e') = Eperm \<sigma> (corec e')"
+"Evalid' e \<Longrightarrow> small \<sigma> \<Longrightarrow> bij \<sigma> \<Longrightarrow>   
+ corec (Eperm' \<sigma> e) = Eperm \<sigma> (corec e)"
 sorry
 
+
 lemma corec_EVrs:
-"EVrs (corec e') \<subseteq> EVrs' e'"
+"Evalid' e \<Longrightarrow> EVrs (corec e) \<subseteq> EVrs' e"
 sorry
 
 lemma corec_unique: 
-assumes "\<And> e U. Edtor' e = Inl U \<Longrightarrow> Gmap H H ` U  \<subseteq> Edtor (H e)"
-and "\<And>e e1. Edtor' e = Inr e1 \<Longrightarrow> H e = e1"
-shows "H = corec"
+assumes "\<And> e U. Evalid' e \<Longrightarrow> Edtor' e = Inl U \<Longrightarrow> Gmap H H ` U  \<subseteq> Edtor (H e)"
+and "\<And>e e1. Evalid' e \<Longrightarrow> Edtor' e = Inr e1 \<Longrightarrow> H e = e1"
+shows "\<And>e. Evalid' e \<Longrightarrow> H e = corec e"
 sorry
 
 end (* locale Comodel *)
