thys/Common_Rec_Corec/Models.thy
@@ -8,31 +8,32 @@ locale Model =
 fixes Ector' :: "('a, 'a, 'a::var P\<Rightarrow>'E','a P\<Rightarrow>'E') G \<Rightarrow> 'a P \<Rightarrow> 'E'" 
 and Eperm' :: "('a::var \<Rightarrow> 'a) \<Rightarrow> 'E' \<Rightarrow> 'E'" 
 and EVrs' ::"'E' \<Rightarrow> 'a::var set" 
-assumes nom: "nom Eperm' EVrs'"
+assumes nom: "nom (\<lambda>e. True) Eperm' EVrs'"
 and ctorPermM: "\<And>u. ctorPermM Ector' Eperm' u"
 and ctorVarsM: "\<And>u. ctorVarsM Ector' EVrs' u"
 begin 
 
 
-definition rec :: "'a E \<Rightarrow> 'a P\<Rightarrow>'E'" where 
+definition rec :: "'a E \<Rightarrow> 'a P \<Rightarrow> 'E'" where 
 "rec = undefined"
 
 lemma rec_Ector:
-shows "GVrs2 u \<inter> PVrs p = {} \<Longrightarrow> 
+"Pvalid p \<Longrightarrow> GVrs2 u \<inter> PVrs p = {} \<Longrightarrow> GVrs2 u \<inter> GVrs1 u = {} \<Longrightarrow>
  rec (Ector u) p = Ector' (Gmap rec rec u) p"
 sorry
 
 lemma rec_Eperm:
-"small \<sigma> \<Longrightarrow> bij \<sigma> \<Longrightarrow>  
+"Pvalid p \<Longrightarrow> small \<sigma> \<Longrightarrow> bij \<sigma> \<Longrightarrow>  
  rec (Eperm \<sigma> e) p = Eperm' \<sigma> (rec e (Pperm (inv \<sigma>) p))"
 sorry
 
 lemma rec_EVrs: 
-"EVrs' (rec e p) \<subseteq> PVrs p \<union> EVrs e"
+"Pvalid p \<Longrightarrow> EVrs' (rec e p) \<subseteq> PVrs p \<union> EVrs e"
 sorry
 
 lemma rec_unique:
-assumes "\<And>u. GVrs2 u \<inter> PVrs p = {} \<Longrightarrow> H (Ector u) p = Ector' (Gmap H H u) p"
+assumes "\<And>u. Pvalid p \<Longrightarrow> GVrs2 u \<inter> PVrs p = {} \<Longrightarrow> GVrs2 u \<inter> GVrs1 u = {} \<Longrightarrow>
+  H (Ector u) p = Ector' (Gmap H H u) p"
 shows "H = rec" 
 sorry
 
